\documentclass{article}

\usepackage[utf8]{inputenc}
\usepackage[spanish]{babel}

\usepackage[sc]{mathpazo}
\linespread{1.05}
\usepackage[T1]{fontenc}

\usepackage{fullpage,amsmath}

\usepackage{graphicx}

\usepackage{array}
\newcolumntype{x}[1]{>{\centering\hspace{0pt}}p{#1}}

\title{NÃºmeros y polinomios de Bernoulli}
\date{}

\begin{document}

\maketitle

\[ S_k (n) = \sum_{1 \le i \le n} i^k = 1^k + 2^k + \cdots + n^k \]

\[ S_k (n) = \frac{1}{k+1} \, \left((n+1)^{k+1} - 1 - \sum_{0 \le i \le k-1} {k+1\choose i} \, S_i (n)\right) \]

\vspace{2em}

\[ \sum_{0 \le i \le k} {k+1 \choose i}\,B_i = k+1 \quad \longleftrightarrow \quad \frac{t\,e^t}{e^t - 1} = \sum_{k \ge 0} B_k \, \frac{t^k}{k!} \]

{\def\arraystretch{1.5}
\[ \begin{array}{rx{0.5cm}x{0.5cm}x{1.2cm}x{0.5cm}x{1.2cm}x{0.5cm}x{1.2cm}x{0.5cm}x{1.2cm}x{0.5cm}x{1.2cm}}
k\colon & $0$ & $1$ & $2$ & $3$ & $4$ & $5$ & $6$ & $7$ & $8$ & $9$ & $10$ \tabularnewline
\hline
B_k\colon & $1$ & $\frac{1}{2}$ & $\frac{1}{6}$ & $0$ & $-\frac{1}{30}$ & $0$ & $\frac{1}{42}$ & $0$ & $-\frac{1}{30}$ & $0$ & $\frac{5}{66}$ \tabularnewline
\hline
k\colon & & $11$ & $12$ & $13$ & $14$ & $15$ & $16$ & $17$ & $18$ & $19$ & $20$ \tabularnewline
\hline
B_k\colon & & $0$ & $-\frac{691}{2730}$ & $0$ & $\frac{7}{6}$ & $0$ & $-\frac{3617}{510}$ & $0$ & $\frac{43867}{798}$ & $0$ & $-\frac{174611}{330}$
\end{array} \]
}

\vspace{2em}

\[ \frac{t\,e^{tx}}{e^t-1} = \sum_{k \ge 0} B_k (x)\,\frac{t^k}{k!} \]

\vspace{2em}

\begin{minipage}[t]{0.5\textwidth}
\[ B_k = S_k' (0) \]

\[ S_k' (x) = k\,S_{k-1} (x) + B_k \]

\[ S_k (x) = \frac{1}{k+1}\,\sum_{0 \le i \le k} {k+1\choose i}\,B_i\,x^{k+1-i} \]
\end{minipage}
\begin{minipage}[t]{0.5\textwidth}
\[ B_k (1) = B_k, ~ B_k (0) = B_k \text{ para } k \ne 1 \]

\[ B_k' (x) = k\,B_{k-1} (x) \]

\[ B_k (x) = \sum_{0 \le i \le k} (-1)^i \, {k \choose i}\,B_i\,x^{k-i} \]
\end{minipage}

\vspace{2em}

\[ B_k (x) = S_k' (x) \text{ para }k\ne 1 \]

\pagebreak

\begin{minipage}[t]{0.5\textwidth}\small
\begin{align*}
S_0 (x) & = x\\
S_1 (x) & = \frac{1}{2}\,x^2\,+\frac{1}{2}\,x\\
S_2 (x) & = \frac{1}{3}\,x^3+\frac{1}{2}\,x^2+\frac{1}{6}\,x\\
S_3 (x) & = \frac{1}{4}\,x^4+\frac{1}{2}\,x^3+\frac{1}{4}\,x^2\\
S_4 (x) & = \frac{1}{5}\,x^5+\frac{1}{2}\,x^4+\frac{1}{3}\,x^3-\frac{1}{30}\,x\\
S_5 (x) & = \frac{1}{6}\,x^6+\frac{1}{2}\,x^5+\frac{5}{12}\,x^4-\frac{1}{12}\,x^2\\
S_6 (x) & = \frac{1}{7}\,x^7+\frac{1}{2}\,x^6+\frac{1}{2}\,x^5-\frac{1}{6}\,x^3+\frac{1}{42}\,x\\
S_7 (x) & = \frac{1}{8}\,x^8+\frac{1}{2}\,x^7+\frac{7}{12}\,x^6-\frac{7}{24}\,x^4+\frac{1}{12}\,x^2\\
S_8 (x) & = \frac{1}{9}\,x^9+\frac{1}{2}\,x^8+\frac{2}{3}\,x^7-\frac{7}{15}\,x^5+\frac{2}{9}\,x^3-\frac{1}{30}\,x\\
S_9 (x) & = \frac{1}{10}\,x^{10}+\frac{1}{2}\,x^9+\frac{3}{4}\,x^8-\frac{7}{10}\,x^6+\frac{1}{2}\,x^4-\frac{3}{20}\,x^2\\
S_{10} (x) & = \frac{1}{11}\,x^{11}+\frac{1}{2}\,x^{10}+\frac{5}{6}\,x^9-x^7+x^5-\frac{1}{2}\,x^3+\frac{5}{66}\,x
\end{align*}
\end{minipage}
\begin{minipage}[t]{0.5\textwidth}\small
\begin{align*}
B_0 (x) & = 1\\
B_1 (x) & = x - \frac{1}{2}\\
B_2 (x) & = x^2 - x + \frac{1}{6}\\
B_3 (x) & = x^3 - \frac{3}{2}\,x^2 + \frac{1}{2}\,x,\\
B_4 (x) & = x^4 - 2\,x^3 + x^2 - \frac{1}{30}\\
B_5 (x) & = x^5 - \frac{5}{2}\,x^4 + \frac{5}{3}\,x^3 - \frac{1}{6}\,x\\
B_6 (x) & = x^6 - 3\,x^5 + \frac{5}{2}\,x^4 - \frac{1}{2}\,x^2 + \frac{1}{42},\\
B_7 (x) & = x^7 - \frac{7}{2}\,x^6 + \frac{7}{2}\,x^5 - \frac{7}{6}\,x^3 + \frac{1}{6}\,x\\
B_8 (x) & = x^8 - 4\,x^7 + \frac{14}{3}\,x^6 - \frac{7}{3}\,x^4 + \frac{2}{3}\,x^2 - \frac{1}{30},\\
B_9 (x) & = x^9 - \frac{9}{2}\,x^8 + 6\,x^7 - \frac{21}{5}\,x^5 + 2\,x^3 - \frac{3}{10}\,x\\
B_{10} (x) & = x^{10} - 5\,x^9 + \frac{15}{2}\,x^8 - 7\,x^6 + 5\,x^4 - \frac{3}{2}\,x^2 + \frac{5}{66}
\end{align*}
\end{minipage}

\vspace{2em}

\begin{center}
\includegraphics{bernpol.mps}
\end{center}

\begin{gather*}
B_k (1-x) = (-1)^k\,B_k (x)\\
\int_0^1 B_k (x)\,dx = 0
\end{gather*}

\end{document}
